02Typed/Typechecking.thy
@@ -20,23 +20,26 @@ primrec erase :: "texpr \<Rightarrow> nexpr" where
 | "erase (TLam x t e) = NLam x (erase e)"
 | "erase (TApp e\<^sub>1 e\<^sub>2) = NApp (erase e\<^sub>1) (erase e\<^sub>2)"
 
-primrec typecheck' :: "subst \<Rightarrow> var set \<Rightarrow> nexpr \<rightharpoonup> 
-    hexpr \<times> uexpr \<times> var set \<times> (uexpr \<times> uexpr) list" where
+definition env_subst :: "subst \<Rightarrow> subst \<Rightarrow> subst" where
+  "env_subst sub \<Gamma> = map_option (subst sub) \<circ> \<Gamma>"
+
+primrec typecheck' :: "subst \<Rightarrow> var set \<Rightarrow> nexpr \<rightharpoonup> hexpr \<times> uexpr \<times> var set \<times> subst" where
   "typecheck' \<Gamma> vs (NVar x) = (case \<Gamma> x of 
-      Some t \<Rightarrow> Some (HVar x, t, vs, []) 
+      Some t \<Rightarrow> Some (HVar x, t, vs, Map.empty) 
     | None \<Rightarrow> None)"
-| "typecheck' \<Gamma> vs (NConst k) = Some (HConst k, Ctor ''Base'' [], vs, [])"
+| "typecheck' \<Gamma> vs (NConst k) = Some (HConst k, Ctor ''Base'' [], vs, Map.empty)"
 | "typecheck' \<Gamma> vs (NLam x e) = (
     let v = fresh vs
     in case typecheck' (\<Gamma>(x \<mapsto> Var v)) (insert v vs) e of
-        Some (e', t, vs', uni) \<Rightarrow> Some (HLam x (Var v) e', Ctor ''Arrow'' [Var v, t], vs', uni)
+        Some (e', t, vs', sub) \<Rightarrow> Some (HLam x (Var v) e', Ctor ''Arrow'' [Var v, t], vs', sub)
       | None \<Rightarrow> None)"
 | "typecheck' \<Gamma> vs (NApp e\<^sub>1 e\<^sub>2) = (
     let v = fresh vs
     in case typecheck' \<Gamma> (insert v vs) e\<^sub>1 of 
-        Some (e\<^sub>1', t\<^sub>1, vs', uni\<^sub>1) \<Rightarrow> (case typecheck' \<Gamma> vs' e\<^sub>2 of
-            Some (e\<^sub>2', t\<^sub>2, vs'', uni\<^sub>2) \<Rightarrow> 
-              Some (HApp e\<^sub>1' e\<^sub>2', Var v, vs'', (t\<^sub>1, Ctor ''arrow'' [t\<^sub>2, Var v]) # uni\<^sub>1 @ uni\<^sub>2)
+        Some (e\<^sub>1', t\<^sub>1, vs', sub\<^sub>1) \<Rightarrow> (case typecheck' (env_subst sub\<^sub>1 \<Gamma>) vs' e\<^sub>2 of
+            Some (e\<^sub>2', t\<^sub>2, vs'', sub\<^sub>2) \<Rightarrow> (case unify t\<^sub>1 (Ctor ''Arrow'' [t\<^sub>2, Var v]) of
+                Some sub\<^sub>3 \<Rightarrow> Some (HApp e\<^sub>1' e\<^sub>2', Var v, vs'', combine_subst sub\<^sub>3 sub\<^sub>2)
+              | None \<Rightarrow> None)
           | None \<Rightarrow> None)
       | None \<Rightarrow> None)"
 
@@ -47,11 +50,15 @@ fun typeify :: "uexpr \<Rightarrow> ty" where
     (if k = ''Arrow'' then Arrow (typeify t\<^sub>1) (typeify t\<^sub>2) else undefined)"
 | "typeify (Ctor k ts) = undefined"
 
-fun valid_ty_uexpr :: "uexpr \<Rightarrow> bool" where
+fun valid_ty_uexpr' :: "string \<Rightarrow> nat \<Rightarrow> bool" where
+  "valid_ty_uexpr' k 0 = (k = ''Base'')"
+| "valid_ty_uexpr' k (Suc 0) = False"
+| "valid_ty_uexpr' k (Suc (Suc 0)) = (k = ''Arrow'')"
+| "valid_ty_uexpr' k (Suc (Suc (Suc x))) = False"
+
+primrec valid_ty_uexpr :: "uexpr \<Rightarrow> bool" where
   "valid_ty_uexpr (Var v) = True"
-| "valid_ty_uexpr (Ctor k []) = (k = ''Base'')"
-| "valid_ty_uexpr (Ctor k [t\<^sub>1, t\<^sub>2]) = (k = ''Arrow'' \<and> valid_ty_uexpr t\<^sub>1 \<and> valid_ty_uexpr t\<^sub>2)"
-| "valid_ty_uexpr (Ctor k ts) = False"
+| "valid_ty_uexpr (Ctor k ts) = (valid_ty_uexpr' k (length ts) \<and> list_all valid_ty_uexpr ts)"
 
 definition valid_ty_uexprs :: "(uexpr \<times> uexpr) list \<Rightarrow> bool" where
   "valid_ty_uexprs ts = list_all (\<lambda>(t\<^sub>1, t\<^sub>2). valid_ty_uexpr t\<^sub>1 \<and> valid_ty_uexpr t\<^sub>2) ts"
@@ -71,13 +78,6 @@ primrec valid_ty_hexpr :: "hexpr \<Rightarrow> bool" where
 | "valid_ty_hexpr (HLam x t e) = (valid_ty_uexpr t \<and> valid_ty_hexpr e)"
 | "valid_ty_hexpr (HApp e\<^sub>1 e\<^sub>2) = (valid_ty_hexpr e\<^sub>1 \<and> valid_ty_hexpr e\<^sub>2)"
 
-fun typecheck :: "nexpr \<rightharpoonup> texpr \<times> ty" where
-  "typecheck e = (case typecheck' Map.empty {} e of
-      Some (e', t, vs, uni) \<Rightarrow> (case unify' uni of 
-          Some sub \<Rightarrow> Some (solidify (hsubst sub e'), typeify (subst sub t))
-        | None \<Rightarrow> None)
-    | None \<Rightarrow> None)"
-
 fun tsubsts :: "subst \<Rightarrow> ty \<Rightarrow> ty" where
   "tsubsts sub (TyVar y) = (case sub y of Some t \<Rightarrow> typeify t | None \<Rightarrow> TyVar y)"
 | "tsubsts sub Base = Base"
@@ -89,11 +89,68 @@ primrec tsubstt :: "subst \<Rightarrow> texpr \<Rightarrow> texpr" where
 | "tsubstt sub (TLam x t e) = TLam x (tsubsts sub t) (tsubstt sub e)"
 | "tsubstt sub (TApp e\<^sub>1 e\<^sub>2) = TApp (tsubstt sub e\<^sub>1) (tsubstt sub e\<^sub>2)"
 
+fun typecheck :: "nexpr \<rightharpoonup> texpr \<times> ty" where
+  "typecheck e = (case typecheck' Map.empty {} e of
+      Some (e', t, vs, sub) \<Rightarrow> Some (tsubstt sub (solidify e'), tsubsts sub (typeify t))
+    | None \<Rightarrow> None)"
+
+lemma typecheck_Some [consumes 1, case_names NVar NConst NLam NApp]: "
+  typecheck' \<Gamma> vs e = Some (e', t, vs', sub) \<Longrightarrow> 
+  (\<And>\<Gamma> vs t x. \<Gamma> x = Some t \<Longrightarrow> P \<Gamma> vs (NVar x) (HVar x) t vs Map.empty) \<Longrightarrow> 
+  (\<And>\<Gamma> vs k. P \<Gamma> vs (NConst k) (HConst k) (Ctor ''Base'' []) vs Map.empty) \<Longrightarrow> 
+  (\<And>\<Gamma> vs vs' sub x e\<^sub>1 e\<^sub>1' t' v. v = fresh vs \<Longrightarrow> typecheck' (\<Gamma>(x \<mapsto> Var v)) (insert v vs) e\<^sub>1 = 
+    Some (e\<^sub>1', t', vs', sub) \<Longrightarrow> P (\<Gamma>(x \<mapsto> Var v)) (insert v vs) e\<^sub>1 e\<^sub>1' t' vs' sub \<Longrightarrow> 
+      P \<Gamma> vs (NLam x e\<^sub>1) (HLam x (Var v) e\<^sub>1') (Ctor ''Arrow'' [Var v, t']) vs' sub) \<Longrightarrow> 
+  (\<And>\<Gamma> vs vs' e\<^sub>1 e\<^sub>2 v e\<^sub>1' t\<^sub>1 vs'' sub\<^sub>1 e\<^sub>2' t\<^sub>2 sub\<^sub>2 sub\<^sub>3. v = fresh vs \<Longrightarrow> 
+    typecheck' \<Gamma> (insert v vs) e\<^sub>1 = Some (e\<^sub>1', t\<^sub>1, vs'', sub\<^sub>1) \<Longrightarrow> 
+      typecheck' (env_subst sub\<^sub>1 \<Gamma>) vs'' e\<^sub>2 = Some (e\<^sub>2', t\<^sub>2, vs', sub\<^sub>2) \<Longrightarrow> 
+        P \<Gamma> (insert v vs) e\<^sub>1 e\<^sub>1' t\<^sub>1 vs'' sub\<^sub>1 \<Longrightarrow> P (env_subst sub\<^sub>1 \<Gamma>) vs'' e\<^sub>2 e\<^sub>2' t\<^sub>2 vs' sub\<^sub>2 \<Longrightarrow> 
+          unify t\<^sub>1 (Ctor ''Arrow'' [t\<^sub>2, Var v]) = Some sub\<^sub>3 \<Longrightarrow> 
+            P \<Gamma> vs (NApp e\<^sub>1 e\<^sub>2) (HApp e\<^sub>1' e\<^sub>2') (Var v) vs' (combine_subst sub\<^sub>3 sub\<^sub>2)) \<Longrightarrow> 
+              P \<Gamma> vs e e' t vs' sub"
+proof (induction e arbitrary: \<Gamma> vs e' t vs' sub)
+  case (NLam x e)
+  let ?v = "fresh vs"
+  from NLam(2) obtain ee' tt where E: "e' = HLam x (Var ?v) ee' \<and> t = Ctor ''Arrow'' [Var ?v, tt] \<and>
+    typecheck' (\<Gamma>(x \<mapsto> Var ?v)) (insert ?v vs) e = Some (ee', tt, vs', sub)" 
+      by (auto simp add: Let_def split: option.splits)
+  with NLam have "P (\<Gamma>(x \<mapsto> Var ?v)) (insert ?v vs) e ee' tt vs' sub" by auto
+  with NLam E show ?case by metis
+qed (auto simp add: Let_def split: option.splits)
+
+lemma typecheck_None [consumes 1, case_names NVar NLam NApp1 NApp2 NApp3]: "
+  typecheck' \<Gamma> vs e = None \<Longrightarrow> 
+  (\<And>\<Gamma> vs x. \<Gamma> x = None \<Longrightarrow> P \<Gamma> vs (NVar x)) \<Longrightarrow> 
+  (\<And>\<Gamma> vs x e\<^sub>1 v. v = fresh vs \<Longrightarrow> typecheck' (\<Gamma>(x \<mapsto> Var v)) (insert v vs) e\<^sub>1 = None \<Longrightarrow> 
+    P (\<Gamma>(x \<mapsto> Var v)) (insert v vs) e\<^sub>1 \<Longrightarrow> P \<Gamma> vs (NLam x e\<^sub>1)) \<Longrightarrow> 
+  (\<And>\<Gamma> vs e\<^sub>1 e\<^sub>2 v. v = fresh vs \<Longrightarrow> typecheck' \<Gamma> (insert v vs) e\<^sub>1 = None \<Longrightarrow> P \<Gamma> (insert v vs) e\<^sub>1 \<Longrightarrow> 
+    P \<Gamma> vs (NApp e\<^sub>1 e\<^sub>2)) \<Longrightarrow> 
+  (\<And>\<Gamma> vs e\<^sub>1 e\<^sub>2 v e\<^sub>1' t\<^sub>1 vs'' sub\<^sub>1. v = fresh vs \<Longrightarrow> 
+    typecheck' \<Gamma> (insert v vs) e\<^sub>1 = Some (e\<^sub>1', t\<^sub>1, vs'', sub\<^sub>1) \<Longrightarrow> 
+      typecheck' (env_subst sub\<^sub>1 \<Gamma>) vs'' e\<^sub>2 = None \<Longrightarrow> P (env_subst sub\<^sub>1 \<Gamma>) vs'' e\<^sub>2 \<Longrightarrow> 
+        P \<Gamma> vs (NApp e\<^sub>1 e\<^sub>2)) \<Longrightarrow> 
+  (\<And>\<Gamma> vs vs' e\<^sub>1 e\<^sub>2 v e\<^sub>1' t\<^sub>1 vs'' sub\<^sub>1 e\<^sub>2' t\<^sub>2 sub\<^sub>2. v = fresh vs \<Longrightarrow> 
+    typecheck' \<Gamma> (insert v vs) e\<^sub>1 = Some (e\<^sub>1', t\<^sub>1, vs'', sub\<^sub>1) \<Longrightarrow> 
+      typecheck' (env_subst sub\<^sub>1 \<Gamma>) vs'' e\<^sub>2 = Some (e\<^sub>2', t\<^sub>2, vs', sub\<^sub>2) \<Longrightarrow> 
+        unify t\<^sub>1 (Ctor ''Arrow'' [t\<^sub>2, Var v]) = None \<Longrightarrow> 
+          P \<Gamma> vs (NApp e\<^sub>1 e\<^sub>2)) \<Longrightarrow> P \<Gamma> vs e"
+proof (induction e arbitrary: \<Gamma> vs)
+  case (NLam x e)
+  let ?v = "fresh vs"
+  from NLam have X: "typecheck' (\<Gamma>(x \<mapsto> Var ?v)) (insert ?v vs) e = None" 
+    by (auto simp add: Let_def split: option.splits)
+  with NLam have "P (\<Gamma>(x \<mapsto> Var ?v)) (insert ?v vs) e" by simp
+  with NLam(4) X show ?case by blast
+qed (simp_all add: Let_def split: option.splits prod.splits)
+
 lemma [simp]: "valid_ty_uexpr t \<Longrightarrow> typeify (subst sub t) = tsubsts sub (typeify t)"
   by (induction t rule: typeify.induct) (simp_all split: option.splits)
 
 lemma [simp]: "valid_ty_subst Map.empty"
   by (simp add: valid_ty_subst_def)
+
+lemma [simp]: "valid_ty_uexpr e \<Longrightarrow> typeify (subst sub e) = tsubsts sub (typeify e)"
+  by (induction e rule: typeify.induct) (auto split: option.splits)
 
 lemma [simp]: "valid_ty_subst \<Gamma> \<Longrightarrow> 
     map_option (typeify \<circ> subst sub) (\<Gamma> x) = map_option (tsubsts sub \<circ> typeify) (\<Gamma> x)"
@@ -104,6 +161,9 @@ lemma [simp]: "valid_ty_subst \<Gamma> \<Longrightarrow>
   by auto
 
 lemma [simp]: "valid_ty_hexpr e \<Longrightarrow> solidify (hsubst sub e) = tsubstt sub (solidify e)"
+  by (induction e) simp_all
+
+lemma [simp]: "erase (solidify (hsubst sub e)) = erase (solidify e)"
   by (induction e) simp_all
 
 lemma [simp]: "erase (tsubstt sub e) = erase e"
@@ -139,14 +199,29 @@ lemma [simp]: "valid_ty_uexpr e \<Longrightarrow> valid_ty_uexprs ess \<Longrigh
   by (induction ess rule: list_subst.induct) (auto simp add: valid_ty_uexprs_def)
 
 lemma [simp]: "valid_ty_uexpr t \<Longrightarrow> valid_ty_subst sub \<Longrightarrow> valid_ty_uexpr (subst sub t)"
-  by (induction t rule: valid_ty_uexpr.induct) 
+  and [simp]: "list_all valid_ty_uexpr ts \<Longrightarrow> valid_ty_subst sub \<Longrightarrow> 
+    list_all valid_ty_uexpr (map (subst sub) ts)"
+  by (induction t and ts rule: vars_varss.induct) 
      (auto simp add: valid_ty_subst_def ran_def split: option.splits)
 
 lemma [elim]: "valid_ty_subst \<Gamma> \<Longrightarrow> \<Gamma> x = Some t \<Longrightarrow> valid_ty_uexpr t"
   by (auto simp add: valid_ty_subst_def ran_def)
 
-lemma [elim]: "valid_ty_uexpr (Ctor k es) \<Longrightarrow> list_all valid_ty_uexpr es"
-  by (induction "Ctor k es" rule: valid_ty_uexpr.induct) auto
+lemma [simp]: "valid_ty_subst \<Gamma> \<Longrightarrow> valid_ty_subst sub\<^sub>2 \<Longrightarrow> 
+  map_option (typeify \<circ> subst sub\<^sub>1 \<circ> subst sub\<^sub>2) (\<Gamma> x) = 
+    map_option (tsubsts sub\<^sub>1 \<circ> tsubsts sub\<^sub>2 \<circ> typeify) (\<Gamma> x)"
+proof (cases "\<Gamma> x")
+  case (Some e)
+  moreover assume "valid_ty_subst \<Gamma>"
+  ultimately have E: "valid_ty_uexpr e" by auto
+  assume "valid_ty_subst sub\<^sub>2"
+  with Some E show ?thesis by simp
+qed simp_all
+
+lemma [simp]: "valid_ty_subst \<Gamma> \<Longrightarrow> valid_ty_subst sub\<^sub>2 \<Longrightarrow> 
+  map_option (typeify \<circ> subst sub\<^sub>1 \<circ> subst sub\<^sub>2) \<circ> \<Gamma> = 
+    map_option (tsubsts sub\<^sub>1 \<circ> tsubsts sub\<^sub>2 \<circ> typeify) \<circ> \<Gamma>"
+  by auto
 
 lemma [elim]: "valid_ty_uexprs ts \<Longrightarrow> unify' ts = Some sub \<Longrightarrow> valid_ty_subst sub"                                  
 proof (induction ts arbitrary: sub rule: unify'.induct)
@@ -193,128 +268,112 @@ proof (induction \<Gamma> e t rule: typecheckn.induct)
   thus ?case by blast
 qed simp_all
 
-lemma [simp]: "valid_ty_subst \<Gamma> \<Longrightarrow> typecheck' \<Gamma> vs e = Some (e', t, vs', uni) \<Longrightarrow> 
-  valid_ty_hexpr e' \<and> valid_ty_uexpr t"
-proof (induction e arbitrary: \<Gamma> vs e' t vs' uni)
-  case (NLam x e)
-  let ?v = "fresh vs"
-  from NLam obtain ee' tt where T: "e' = HLam x (Var ?v) ee' \<and> 
-    t = Ctor ''Arrow'' [Var ?v, tt] \<and> 
-      typecheck' (\<Gamma>(x \<mapsto> Var ?v)) (insert ?v vs) e = Some (ee', tt, vs', uni)" 
-    by (auto simp add: Let_def split: option.splits)
-  from NLam have "valid_ty_subst (\<Gamma>(x \<mapsto> Var ?v))" by simp
-  with NLam T have "valid_ty_uexpr tt \<and> valid_ty_hexpr ee'" by blast
-  with NLam have "valid_ty_uexpr (Ctor ''Arrow'' [Var ?v, tt]) \<and> 
-    valid_ty_hexpr (HLam x (Var ?v) ee')" by simp
-  with T show ?case by blast
-qed (auto simp add: Let_def split: option.splits)
+lemma valid_ty_uexpr_structrual [simp]: "structural valid_ty_uexpr"
+  by (auto simp add: structural_def)
 
-lemma [elim]: "valid_ty_subst \<Gamma> \<Longrightarrow> typecheck' \<Gamma> vs e = Some (e', t, vs', uni) \<Longrightarrow> valid_ty_uexpr t"
+lemma [simp]: "valid_ty_subst sub \<Longrightarrow> valid_ty_subst \<Gamma> \<Longrightarrow> valid_ty_subst (env_subst sub \<Gamma>)"
+  by (auto simp add: valid_ty_subst_def env_subst_def ran_def)
+
+lemma [simp]: "valid_ty_subst s1 \<Longrightarrow> valid_ty_subst s2 \<Longrightarrow> valid_ty_subst (combine_subst s1 s2)"
+proof (unfold valid_ty_subst_def combine_subst_def ran_def, rule)
+  fix x
+  assume S1: "\<forall>x \<in> {b. \<exists>a. s1 a = Some b}. valid_ty_uexpr x"
+  assume S2: "\<forall>x \<in> {b. \<exists>a. s2 a = Some b}. valid_ty_uexpr x"
+  assume "x \<in> {b. \<exists>a. (case s2 a of None \<Rightarrow> s1 a | Some e \<Rightarrow> Some (subst s1 e)) = Some b}"
+  then obtain y where Y: "(case s2 y of None \<Rightarrow> s1 y | Some e \<Rightarrow> Some (subst s1 e)) = Some x" 
+    by auto
+  from S1 S2 Y show "valid_ty_uexpr x" 
+  proof (cases "s2 y")
+    case (Some e)
+    from S1 have "valid_ty_subst s1" by (auto simp add: valid_ty_subst_def ran_def)
+    with S2 Y Some show ?thesis by auto
+  qed auto
+qed
+
+lemma [simp]: "hsubst (combine_subst s t) e = hsubst s (hsubst t e)"
+  by (induction e) simp_all
+
+lemma [simp]: "typecheck' \<Gamma> vs e = Some (e', t, vs', sub) \<Longrightarrow> valid_ty_subst \<Gamma> \<Longrightarrow>  
+  valid_ty_hexpr e' \<and> valid_ty_uexpr t \<and> valid_ty_subst sub"
+proof (induction rule: typecheck_Some)
+  case (NApp \<Gamma> vs vs' e\<^sub>1 e\<^sub>2 v e\<^sub>1' t\<^sub>1 vs'' sub\<^sub>1 e\<^sub>2' t\<^sub>2 sub\<^sub>2 sub\<^sub>3)
+  hence "valid_ty_uexpr (Ctor ''Arrow'' [t\<^sub>2, Var v])" by simp
+  with NApp have X: "valid_ty_subst sub\<^sub>3" by fastforce
+  hence "valid_ty_uexpr (case sub\<^sub>3 v of None \<Rightarrow> Var v | Some e \<Rightarrow> e)" 
+    by (auto simp add: valid_ty_subst_def ran_def split: option.splits)
+  with NApp X show ?case by auto
+qed fastforce+
+
+lemma [elim]: "valid_ty_subst \<Gamma> \<Longrightarrow> typecheck' \<Gamma> vs e = Some (e', t, vs', sub) \<Longrightarrow> valid_ty_uexpr t"
   by simp
 
-lemma [elim]: "valid_ty_subst \<Gamma> \<Longrightarrow> typecheck' \<Gamma> vs e = Some (e', t, vs', uni) \<Longrightarrow> 
+lemma [elim]: "valid_ty_subst \<Gamma> \<Longrightarrow> typecheck' \<Gamma> vs e = Some (e', t, vs', sub) \<Longrightarrow> 
     valid_ty_hexpr e'"
   by simp
 
-lemma typecheck_succeeds [simp]: "typecheck' \<Gamma> vs e = Some (e', t, vs', uni) \<Longrightarrow> 
-  unify' uni = Some sub \<Longrightarrow> 
+lemma [elim]: "valid_ty_subst \<Gamma> \<Longrightarrow> typecheck' \<Gamma> vs e = Some (e', t, vs', sub) \<Longrightarrow> 
+    valid_ty_subst sub"
+  by simp
+
+lemma typecheck_succeeds [simp]: "typecheck' \<Gamma> vs e = Some (e', t, vs', sub) \<Longrightarrow> 
+  valid_ty_subst \<Gamma> \<Longrightarrow>
     map_option (typeify \<circ> subst sub) \<circ> \<Gamma> \<turnstile>\<^sub>n solidify (hsubst sub e') : typeify (subst sub t)"
-proof (induction e arbitrary: \<Gamma> vs e' t vs' uni sub)
-  case (NVar x)
-  hence T: "\<Gamma> x = Some t \<and> e' = HVar x \<and> vs' = vs \<and> uni = []" by (simp split: option.splits)
-  moreover with NVar have "sub = Map.empty" by simp
-  moreover from T have "map_option (typeify \<circ> subst Map.empty) \<circ> \<Gamma> \<turnstile>\<^sub>n 
-    solidify (hsubst Map.empty (HVar x)) : typeify (subst Map.empty t)" by simp
-  ultimately show ?case by blast
-next
-  case (NConst k)
-  hence "e' = HConst k \<and> t = Ctor ''Base'' [] \<and> vs' = vs \<and> uni = []" by simp
-  hence "map_option (typeify \<circ> subst sub) \<circ> \<Gamma> \<turnstile>\<^sub>n solidify (hsubst sub e') : typeify (subst sub t)" 
-    by simp
+proof (induction rule: typecheck_Some)
+  case (NLam \<Gamma> vs vs' sub x e\<^sub>1 e\<^sub>1' t' v)
+  hence "valid_ty_subst (\<Gamma>(x \<mapsto> Var v))" by simp
+  with NLam have "map_option (typeify \<circ> subst sub) \<circ> \<Gamma>(x \<mapsto> Var v) \<turnstile>\<^sub>n solidify (hsubst sub e\<^sub>1') : 
+    typeify (subst sub t')" by blast
+  hence "map_option (typeify \<circ> subst sub) \<circ> \<Gamma> \<turnstile>\<^sub>n solidify (hsubst sub (HLam x (Var v) e\<^sub>1')) :
+    typeify (subst sub (Ctor ''Arrow'' [Var v, t']))" by simp
   thus ?case by blast
 next
-  case (NLam x e)
-  let ?v = "fresh vs"
-  from NLam obtain ee' tt where T: "e' = HLam x (Var ?v) ee' \<and> t = Ctor ''Arrow'' [Var ?v, tt] \<and>
-    typecheck' (\<Gamma>(x \<mapsto> Var ?v)) (insert ?v vs) e = Some (ee', tt, vs', uni)" 
-      by (auto simp add: Let_def split: option.splits)
-  thus ?case 
-  proof (cases "sub ?v")
-    case None
-    from NLam T have "map_option (typeify \<circ> subst sub) \<circ> (\<Gamma>(x \<mapsto> Var ?v)) \<turnstile>\<^sub>n 
-      solidify (hsubst sub ee') : typeify (subst sub tt)" by blast
-    with None have "map_option (typeify \<circ> subst sub) \<circ> \<Gamma> \<turnstile>\<^sub>n 
-      solidify (hsubst sub (HLam x (Var ?v) ee')) : 
-        typeify (subst sub (Ctor ''Arrow'' [Var ?v, tt]))" by simp
-    with T show ?thesis by blast
-  next
-    case (Some t')
-    from NLam T have "map_option (typeify \<circ> subst sub) \<circ> (\<Gamma>(x \<mapsto> Var ?v)) \<turnstile>\<^sub>n 
-      solidify (hsubst sub ee') : typeify (subst sub tt)" by blast
-    with Some have "map_option (typeify \<circ> subst sub) \<circ> \<Gamma> \<turnstile>\<^sub>n 
-      solidify (hsubst sub (HLam x (Var ?v) ee')) : 
-        typeify (subst sub (Ctor ''Arrow'' [Var ?v, tt]))" by simp
-    with T show ?thesis by blast
-  qed
-next
-  case (NApp e\<^sub>1 e\<^sub>2)
-  let ?v = "fresh vs"
-  from NApp obtain e\<^sub>1' t\<^sub>1 vs'' uni\<^sub>1 e\<^sub>2' t\<^sub>2 uni\<^sub>2 where E: "e' = HApp e\<^sub>1' e\<^sub>2' \<and> t = Var ?v \<and>
-    typecheck' \<Gamma> (insert ?v vs) e\<^sub>1 = Some (e\<^sub>1', t\<^sub>1, vs'', uni\<^sub>1) \<and>
-      typecheck' \<Gamma> vs'' e\<^sub>2 = Some (e\<^sub>2', t\<^sub>2, vs', uni\<^sub>2) \<and> 
-        uni = (t\<^sub>1, Ctor ''arrow'' [t\<^sub>2, Var ?v]) # uni\<^sub>1 @ uni\<^sub>2" 
-    by (auto simp add: Let_def split: option.splits)
+  case (NApp \<Gamma> vs vs' e\<^sub>1 e\<^sub>2 v e\<^sub>1' t\<^sub>1 vs'' sub\<^sub>1 e\<^sub>2' t\<^sub>2 sub\<^sub>2 sub\<^sub>3)
+  from NApp have "v = fresh vs" by simp
+  from NApp have "typecheck' \<Gamma> (insert v vs) e\<^sub>1 = Some (e\<^sub>1', t\<^sub>1, vs'', sub\<^sub>1)" by simp
+  with NApp have E1: "valid_ty_hexpr e\<^sub>1' \<and> valid_ty_subst sub\<^sub>1" by auto
+  from NApp have "typecheck' (env_subst sub\<^sub>1 \<Gamma>) vs'' e\<^sub>2 = Some (e\<^sub>2', t\<^sub>2, vs', sub\<^sub>2)" by simp
+  with NApp have E2: "valid_ty_hexpr e\<^sub>2' \<and> valid_ty_subst sub\<^sub>2" by auto
+  from NApp have "unify t\<^sub>1 (Ctor ''Arrow'' [t\<^sub>2, Var v]) = Some sub\<^sub>3" by simp
+  from NApp have "map_option (typeify \<circ> subst sub\<^sub>1) \<circ> \<Gamma> \<turnstile>\<^sub>n solidify (hsubst sub\<^sub>1 e\<^sub>1') : typeify (subst sub\<^sub>1 t\<^sub>1)" by blast
+  from NApp have "valid_ty_subst \<Gamma>" by simp
+
+  from NApp E1 have "valid_ty_subst (env_subst sub\<^sub>1 \<Gamma>)" by simp
+  with NApp have "map_option (typeify \<circ> subst sub\<^sub>2) \<circ> env_subst sub\<^sub>1 \<Gamma> \<turnstile>\<^sub>n solidify (hsubst sub\<^sub>2 e\<^sub>2') : typeify (subst sub\<^sub>2 t\<^sub>2)" by blast
 
 
-  from NApp E have "unify' uni\<^sub>1 = Some sub\<^sub>1 \<Longrightarrow> 
-    map_option (typeify \<circ> subst sub\<^sub>1) \<circ> \<Gamma> \<turnstile>\<^sub>n solidify (hsubst sub\<^sub>1 e\<^sub>1') : typeify (subst sub\<^sub>1 t\<^sub>1)" by blast
-  from NApp E have "unify' uni\<^sub>2 = Some sub\<^sub>2 \<Longrightarrow> 
-    map_option (typeify \<circ> subst sub\<^sub>2) \<circ> \<Gamma> \<turnstile>\<^sub>n solidify (hsubst sub\<^sub>2 e\<^sub>2') : typeify (subst sub\<^sub>2 t\<^sub>2)" by blast
-
-  from NApp have "unify' uni = Some sub" by simp
-
+  from E1 have X: "map_option (tsubsts sub\<^sub>3 \<circ> tsubsts sub\<^sub>2 \<circ> typeify) \<circ> \<Gamma> \<turnstile>\<^sub>n solidify (hsubst sub\<^sub>3 (hsubst sub\<^sub>2 e\<^sub>1')) : 
+    Arrow xt\<^sub>1 (typeify (subst sub\<^sub>3 (subst sub\<^sub>2 (Var v))))" by simp
+  with NApp E2 have X: "map_option (typeify \<circ> subst sub\<^sub>3 \<circ> subst sub\<^sub>2) \<circ> \<Gamma> \<turnstile>\<^sub>n 
+    solidify (hsubst sub\<^sub>3 (hsubst sub\<^sub>2 e\<^sub>1')) : Arrow xt\<^sub>1 (typeify (subst sub\<^sub>3 (subst sub\<^sub>2 (Var v))))" 
+      by simp
 
 
-  have X: "map_option (typeify \<circ> subst sub) \<circ> \<Gamma> \<turnstile>\<^sub>n solidify (hsubst sub e\<^sub>1') : 
-    Arrow (typeify (subst sub t\<^sub>1)) (typeify (subst sub t))" by simp
-
-
-
-
-  have "map_option (typeify \<circ> subst sub) \<circ> \<Gamma> \<turnstile>\<^sub>n solidify (hsubst sub e\<^sub>2') : typeify (subst sub t\<^sub>1)" 
+  from E2 have "map_option (tsubsts sub\<^sub>3 \<circ> tsubsts sub\<^sub>2 \<circ> typeify) \<circ> \<Gamma> \<turnstile>\<^sub>n tsubstt sub\<^sub>3 (tsubstt sub\<^sub>2 (solidify e\<^sub>2')) : xt\<^sub>1" 
     by simp
-  with X have "map_option (typeify \<circ> subst sub) \<circ> \<Gamma> \<turnstile>\<^sub>n solidify (hsubst sub (HApp e\<^sub>1' e\<^sub>2')) : 
-    typeify (subst sub t)" by simp
-  with E show ?case by blast
-qed
+  with NApp E2 have "map_option (typeify \<circ> subst sub\<^sub>3 \<circ> subst sub\<^sub>2) \<circ> \<Gamma> \<turnstile>\<^sub>n 
+    tsubstt sub\<^sub>3 (tsubstt sub\<^sub>2 (solidify e\<^sub>2')) : xt\<^sub>1" by simp
+  with X E1 E2 have "map_option (typeify \<circ> subst (combine_subst sub\<^sub>3 sub\<^sub>2)) \<circ> \<Gamma> \<turnstile>\<^sub>n 
+    solidify (hsubst (combine_subst sub\<^sub>3 sub\<^sub>2) (HApp e\<^sub>1' e\<^sub>2')) :
+      typeify (subst (combine_subst sub\<^sub>3 sub\<^sub>2) (Var v))" by (simp add: comp_assoc)
+  thus ?case by blast
+qed simp_all
 
 lemma [simp]: "typecheck e = Some (e\<^sub>t, t) \<Longrightarrow> Map.empty \<turnstile>\<^sub>n e\<^sub>t : t"
 proof -
   assume "typecheck e = Some (e\<^sub>t, t)"
-  then obtain e' tt vs uni sub where "typecheck' Map.empty {} e = Some (e', tt, vs, uni) \<and>
-    unify' uni = Some sub \<and> e\<^sub>t = solidify (hsubst sub e') \<and> t = typeify (subst sub tt)" 
-      by (auto split: option.splits)
+  then obtain e' tt vs sub where T: "typecheck' Map.empty {} e = Some (e', tt, vs, sub) \<and>
+    e\<^sub>t = tsubstt sub (solidify e') \<and> t = tsubsts sub (typeify tt)" by (auto split: option.splits)
   moreover hence "map_option (typeify \<circ> subst sub) \<circ> Map.empty \<turnstile>\<^sub>n solidify (hsubst sub e') : 
     typeify (subst sub tt)" by (metis typecheck_succeeds)
+  moreover from T have "valid_ty_uexpr tt" and "valid_ty_hexpr e'" by auto
   ultimately show "Map.empty \<turnstile>\<^sub>n e\<^sub>t : t" by simp
 qed
 
-lemma erase_solidify [simp]: "typecheck' \<Gamma> vs e = Some (e', t, vs', uni) \<Longrightarrow> 
-    e = erase (solidify e')"
-  by (induction e arbitrary: \<Gamma> vs e' t vs' uni) 
-     (auto simp add: Let_def split: option.splits)
+lemma [simp]: "typecheck' \<Gamma> vs e = Some (e', t, vs', sub) \<Longrightarrow> e = erase (solidify e')"
+  by (induction rule: typecheck_Some) auto
 
 lemma [simp]: "typecheck e = Some (e\<^sub>t, t) \<Longrightarrow> e = erase e\<^sub>t"
-proof -
-  assume "typecheck e = Some (e\<^sub>t, t)"
-  then obtain e' tt vs uni sub where T: "typecheck' Map.empty {} e = Some (e', tt, vs, uni) \<and> 
-    unify' uni = Some sub \<and> e\<^sub>t = solidify (hsubst sub e') \<and> t = typeify (subst sub tt)" 
-      by (auto split: option.splits)
-  hence X: "e = erase (solidify e')" by (metis erase_solidify)
-  have "valid_ty_subst Map.empty" by simp
-  with T have "valid_ty_hexpr e'" by fastforce
-  with T X show ?thesis by simp
-qed
+  by (auto split: option.splits)
 
 lemma [dest]: "erase e\<^sub>t = NVar x \<Longrightarrow> e\<^sub>t = TVar x"
   by (induction e\<^sub>t) simp_all
@@ -322,45 +381,37 @@ lemma [dest]: "erase e\<^sub>t = NVar x \<Longrightarrow> e\<^sub>t = TVar x"
 lemma [dest]: "erase e\<^sub>t = NLam x e \<Longrightarrow> \<exists>t e\<^sub>t'. e\<^sub>t = TLam x t e\<^sub>t' \<and> e = erase e\<^sub>t'"
   by (induction e\<^sub>t) simp_all
 
+lemma [dest]: "erase e\<^sub>t = NApp e\<^sub>1 e\<^sub>2 \<Longrightarrow> \<exists>e\<^sub>1' e\<^sub>2'. e\<^sub>t = TApp e\<^sub>1' e\<^sub>2' \<and> e\<^sub>1 = erase e\<^sub>1'\<and> e\<^sub>2 = erase e\<^sub>2'"
+  by (induction e\<^sub>t) simp_all
+
 lemma typecheck_fails' [simp]: "typecheck' \<Gamma> vs e = None \<Longrightarrow> map_option typeify \<circ> \<Gamma> \<turnstile>\<^sub>n e\<^sub>t : t \<Longrightarrow> 
   erase e\<^sub>t = e \<Longrightarrow> False"
-proof (induction e arbitrary: \<Gamma> vs e\<^sub>t t)
-  case (NVar x)
-  hence "\<Gamma> x = None" by (simp split: option.splits)
-  moreover from NVar have "(map_option typeify \<circ> \<Gamma>) x = Some t" by blast
-  ultimately show ?case by simp
+proof (induction arbitrary: e\<^sub>t t rule: typecheck_None)
+  case (NLam \<Gamma> vs x e v)
+  then obtain t\<^sub>1 e\<^sub>t' where E: "e\<^sub>t = TLam x t\<^sub>1 e\<^sub>t' \<and> e = erase e\<^sub>t'" by auto
+  with NLam obtain t\<^sub>2 where T: "((map_option typeify \<circ> \<Gamma>)(x \<mapsto> t\<^sub>1) \<turnstile>\<^sub>n e\<^sub>t' : t\<^sub>2) \<and> t = Arrow t\<^sub>1 t\<^sub>2" 
+    by blast
+
+
+
+
+  from T have "(map_option typeify \<circ> \<Gamma>(x \<mapsto> Var v) \<turnstile>\<^sub>n xe\<^sub>t' : xt) \<and> erase xe\<^sub>t' = e" by simp
+  with NLam E show ?case by blast
 next
-  case (NLam x e)
-  let ?v = "fresh vs"
-  from NLam have T: "typecheck' (\<Gamma>(x \<mapsto> Var ?v)) (insert ?v vs) e = None" 
-    by (auto simp add: Let_def split: option.splits)
-  from NLam obtain t\<^sub>1 e\<^sub>t' where E: "e\<^sub>t = TLam x t\<^sub>1 e\<^sub>t' \<and> e = erase e\<^sub>t'" by auto
-  with NLam obtain t\<^sub>2 where "t = Arrow t\<^sub>1 t\<^sub>2 \<and> (map_option typeify \<circ> \<Gamma>)(x \<mapsto> t\<^sub>1) \<turnstile>\<^sub>n e\<^sub>t' : t\<^sub>2" by blast
-  hence "map_option typeify \<circ> (\<Gamma>(x \<mapsto> Var ?v)) \<turnstile>\<^sub>n e\<^sub>t' : t\<^sub>2" by simp
-  with NLam T E show ?case by blast
-next
-  case (NApp e1 e2)
+  case (NApp2 \<Gamma> vs e\<^sub>1 e\<^sub>2 v e\<^sub>1' t\<^sub>1 vs'' sub\<^sub>1)
   thus ?case by simp
-qed simp_all
+next
+  case (NApp3 \<Gamma> vs vs' e\<^sub>1 e\<^sub>2 v e\<^sub>1' t\<^sub>1 vs'' sub\<^sub>1 e\<^sub>2' t\<^sub>2 sub\<^sub>2)
+  thus ?case by simp
+qed fastforce+
 
 lemma typecheck_fails [simp]: "typecheck e = None \<Longrightarrow> \<nexists>e\<^sub>t t. (Map.empty \<turnstile>\<^sub>n e\<^sub>t : t) \<and> e = erase e\<^sub>t"
-proof (rule, cases "typecheck' Map.empty {} e")
-  case None
+proof 
+  assume "typecheck e = None"
+  hence X: "typecheck' Map.empty {} e = None" by (auto split: option.splits)
   assume "\<exists>e\<^sub>t t. (Map.empty \<turnstile>\<^sub>n e\<^sub>t : t) \<and> e = erase e\<^sub>t"
-  then obtain e\<^sub>t tt where "(map_option typeify \<circ> Map.empty \<turnstile>\<^sub>n e\<^sub>t : tt) \<and> e = erase e\<^sub>t" by fastforce
-  with None show "False" by (metis typecheck_fails')
-next
-  case (Some out)
-  moreover assume "typecheck e = None"
-  ultimately obtain e' t vs uni where X: "typecheck' Map.empty {} e = Some (e', t, vs, uni) \<and> 
-    unify' uni = None" by (auto split: option.splits prod.splits)
-
-
-  assume "\<exists>e\<^sub>t t. (Map.empty \<turnstile>\<^sub>n e\<^sub>t : t) \<and> e = erase e\<^sub>t"
-  then obtain e\<^sub>t tt where "(map_option typeify \<circ> Map.empty \<turnstile>\<^sub>n e\<^sub>t : tt) \<and> e = erase e\<^sub>t" by fastforce
-
-
-  with Some X show "False" by simp
+  then obtain e\<^sub>t t where "(map_option typeify \<circ> Map.empty \<turnstile>\<^sub>n e\<^sub>t : t) \<and> e = erase e\<^sub>t" by fastforce
+  with X show "False" by (metis typecheck_fails')
 qed
 
 lemma [simp]: "valn (erase e) = valt e"
@@ -390,44 +441,36 @@ lemma [simp]: "tsubstt sub (substt x v e) = substt x (tsubstt sub v) (tsubstt su
 lemma [simp]: "e \<Down>\<^sub>t v \<Longrightarrow> tsubstt sub e \<Down>\<^sub>t tsubstt sub v"
   by (induction e v rule: evalt.induct) simp_all
 
-lemma correctness' [simp]: "e \<Down> v \<Longrightarrow> typecheck' \<Gamma> vs e = Some (e\<^sub>t, t1, vs1, uni1) \<Longrightarrow> 
-  typecheck' \<Gamma> vs v = Some (v\<^sub>t, t2, vs2, uni2) \<Longrightarrow> valid_ty_subst \<Gamma> \<Longrightarrow> unify' uni1 = Some sub1 \<Longrightarrow> 
-    unify' uni2 = Some sub2 \<Longrightarrow> typeify (subst sub1 t1) = typeify (subst sub2 t2) \<Longrightarrow> 
-      solidify (hsubst sub1 e\<^sub>t) \<Down>\<^sub>t solidify (hsubst sub2 v\<^sub>t)"
-proof (induction e v arbitrary: vs e\<^sub>t t1 vs1 uni1 v\<^sub>t t2 vs2 uni2 sub1 sub2 rule: evaln.induct)
+lemma correctness' [simp]: "e \<Down> v \<Longrightarrow> typecheck' \<Gamma> vs e = Some (e\<^sub>t, t1, vs1, sub1) \<Longrightarrow> 
+  typecheck' \<Gamma> vs v = Some (v\<^sub>t, t2, vs2, sub2) \<Longrightarrow> valid_ty_subst \<Gamma> \<Longrightarrow> 
+    tsubsts sub1 (typeify t1) = tsubsts sub2 (typeify t2) \<and> 
+      tsubstt sub1 (solidify e\<^sub>t) \<Down>\<^sub>t tsubstt sub2 (solidify v\<^sub>t)"
+proof (induction e v arbitrary: vs e\<^sub>t t1 vs1 sub1 v\<^sub>t t2 vs2 sub2 rule: evaln.induct)
   case (evn_app e\<^sub>1 x e\<^sub>1' e\<^sub>2 v\<^sub>2 v)
   let ?v = "fresh vs"
-  from evn_app obtain e\<^sub>t\<^sub>1 t\<^sub>1 vs'' uni\<^sub>1 e\<^sub>t\<^sub>2 t\<^sub>2 uni\<^sub>2 where E: "e\<^sub>t = HApp e\<^sub>t\<^sub>1 e\<^sub>t\<^sub>2 \<and> t1 = Var ?v \<and>
-    typecheck' \<Gamma> (insert ?v vs) e\<^sub>1 = Some (e\<^sub>t\<^sub>1, t\<^sub>1, vs'', uni\<^sub>1) \<and>
-      typecheck' \<Gamma> vs'' e\<^sub>2 = Some (e\<^sub>t\<^sub>2, t\<^sub>2, vs1, uni\<^sub>2) \<and> 
-        uni1 = (t\<^sub>1, Ctor ''arrow'' [t\<^sub>2, Var ?v]) # uni\<^sub>1 @ uni\<^sub>2" 
+  from evn_app obtain e\<^sub>1'' t\<^sub>1 vs' sub\<^sub>1 e\<^sub>2' t\<^sub>2 sub\<^sub>2 sub\<^sub>3 where E: "e\<^sub>t = HApp e\<^sub>1'' e\<^sub>2' \<and> t1 = Var ?v \<and> 
+    typecheck' \<Gamma> (insert ?v vs) e\<^sub>1 = Some (e\<^sub>1'', t\<^sub>1, vs', sub\<^sub>1) \<and> sub1 = combine_subst sub\<^sub>3 sub\<^sub>2 \<and> 
+      typecheck' (env_subst sub\<^sub>1 \<Gamma>) vs' e\<^sub>2 = Some (e\<^sub>2', t\<^sub>2, vs1, sub\<^sub>2) \<and> 
+        unify t\<^sub>1 (Ctor ''Arrow'' [t\<^sub>2, Var ?v]) = Some sub\<^sub>3" 
     by (auto simp add: Let_def split: option.splits)
+
 
   from evn_app have "e\<^sub>1 \<Down> NLam x e\<^sub>1'" by simp
   from evn_app have "e\<^sub>2 \<Down> v\<^sub>2" by simp
   from evn_app have "substn x v\<^sub>2 e\<^sub>1' \<Down> v" by simp
-  from evn_app E have "typecheck' \<Gamma> (insert ?v vs) (NLam x e\<^sub>1') = Some (xv\<^sub>t, xt20, xvs20, xuni20) \<Longrightarrow>
-    unify' uni\<^sub>1 = Some xsub1 \<Longrightarrow>
-    unify' xuni20 = Some xsub2 \<Longrightarrow>
-    typeify (subst xsub1 t\<^sub>1) = typeify (subst xsub2 xt20) \<Longrightarrow> solidify (hsubst xsub1 e\<^sub>t\<^sub>1) \<Down>\<^sub>t solidify (hsubst xsub2 xv\<^sub>t)" by blast
-  from evn_app have "typecheck' \<Gamma> xvs e\<^sub>2 = Some (xe\<^sub>t, xt10, xvs10, xuni10) \<Longrightarrow>
-    typecheck' \<Gamma> xvs v\<^sub>2 = Some (xv\<^sub>t, xt20, xvs20, xuni20) \<Longrightarrow>
-    unify' xuni10 = Some xsub1 \<Longrightarrow>
-    unify' xuni20 = Some xsub2 \<Longrightarrow>
-    typeify (subst xsub1 xt10) = typeify (subst xsub2 xt20) \<Longrightarrow> solidify (hsubst xsub1 xe\<^sub>t) \<Down>\<^sub>t solidify (hsubst xsub2 xv\<^sub>t)" by simp
-  from evn_app have "typecheck' \<Gamma> xvs (substn x v\<^sub>2 e\<^sub>1') = Some (xe\<^sub>t, xt10, xvs10, xuni10) \<Longrightarrow>
-    typecheck' \<Gamma> xvs v = Some (xv\<^sub>t, xt20, xvs20, xuni20) \<Longrightarrow>
-    unify' xuni10 = Some xsub1 \<Longrightarrow>
-    unify' xuni20 = Some xsub2 \<Longrightarrow>
-    typeify (subst xsub1 xt10) = typeify (subst xsub2 xt20) \<Longrightarrow> solidify (hsubst xsub1 xe\<^sub>t) \<Down>\<^sub>t solidify (hsubst xsub2 xv\<^sub>t)" by simp
-  from evn_app have "typecheck' \<Gamma> vs v = Some (v\<^sub>t, t2, vs2, uni2)" by simp
+  from evn_app E have "typecheck' \<Gamma> (insert ?v vs) (NLam x e\<^sub>1') = Some (xv\<^sub>t, xt20, xvs20, xsub2) \<Longrightarrow>
+    tsubsts sub\<^sub>1 (typeify t\<^sub>1) = tsubsts xsub2 (typeify xt20) \<and> tsubstt sub\<^sub>1 (solidify e\<^sub>1'') \<Down>\<^sub>t tsubstt xsub2 (solidify xv\<^sub>t)" by simp
+  from evn_app have "typecheck' \<Gamma> xvs e\<^sub>2 = Some (xe\<^sub>t, xt10, xvs10, xsub1) \<Longrightarrow>
+    typecheck' \<Gamma> xvs v\<^sub>2 = Some (xv\<^sub>t, xt20, xvs20, xsub2) \<Longrightarrow>
+    tsubsts xsub1 (typeify xt10) = tsubsts xsub2 (typeify xt20) \<and> tsubstt xsub1 (solidify xe\<^sub>t) \<Down>\<^sub>t tsubstt xsub2 (solidify xv\<^sub>t)" by simp
+  from evn_app have "typecheck' \<Gamma> xvs (substn x v\<^sub>2 e\<^sub>1') = Some (xe\<^sub>t, xt10, xvs10, xsub1) \<Longrightarrow>
+    typecheck' \<Gamma> xvs v = Some (xv\<^sub>t, xt20, xvs20, xsub2) \<Longrightarrow>
+    tsubsts xsub1 (typeify xt10) = tsubsts xsub2 (typeify xt20) \<and> tsubstt xsub1 (solidify xe\<^sub>t) \<Down>\<^sub>t tsubstt xsub2 (solidify xv\<^sub>t)" by simp
+  from evn_app have "typecheck' \<Gamma> vs v = Some (v\<^sub>t, t2, vs2, sub2)" by simp
   from evn_app have "valid_ty_subst \<Gamma>" by simp
-  from evn_app have "unify' uni1 = Some sub1" by simp
-  from evn_app have "unify' uni2 = Some sub2" by simp
-  from evn_app have "typeify (subst sub1 t1) = typeify (subst sub2 t2)" by simp
 
 
-  have "solidify (hsubst sub1 e\<^sub>t) \<Down>\<^sub>t solidify (hsubst sub2 v\<^sub>t)" by simp
+  have "tsubsts sub1 (typeify t1) = tsubsts sub2 (typeify t2) \<and> tsubstt sub1 (solidify e\<^sub>t) \<Down>\<^sub>t tsubstt sub2 (solidify v\<^sub>t)" by simp
   thus ?case by simp
 qed (auto simp add: Let_def split: option.splits prod.splits)
 
